missed a simp lemma

src/certigrad/env.lean
@@ -5,36 +5,99 @@ Author: Daniel Selsam
 
 Environments.
 -/
-import .tensor .id library_dev_extras.util library_dev_extras.dmap .reference
+import data.hash_map library_dev.data.list.sort .tensor .id library_dev_extras.util library_dev_extras.dmap .reference
 
 namespace certigrad
 
--- We wrap `dmap` as `env` to avoid the need for higher-order unification.
-@[reducible] def env : Type := dmap reference (λ (ref : reference), T ref.2)
+@[reducible] def pre_env : Type := hash_map reference (λ (ref : reference), T ref.2)
+
+namespace pre_env
+
+definition eqv (m₁ m₂ : pre_env) : Prop :=
+∀ (ref : reference), m₁^.find ref = m₂^.find ref
+
+local infix ~ := eqv
+
+definition eqv.refl (m : pre_env) : m ~ m :=
+assume ref, rfl
+
+definition eqv.symm (m₁ m₂ : pre_env) : m₁ ~ m₂ → m₂ ~ m₁ :=
+assume H ref, eq.symm (H ref)
+
+definition eqv.trans (m₁ m₂ m₃ : pre_env) : m₁ ~ m₂ → m₂ ~ m₃ → m₁ ~ m₃ :=
+assume H₁ H₂ ref, eq.trans (H₁ ref) (H₂ ref)
+
+instance pdmap.eqv_setoid : setoid pre_env :=
+setoid.mk eqv (mk_equivalence eqv eqv.refl eqv.symm eqv.trans)
+
+end pre_env
+
+def env : Type := quot pre_env.eqv
 
 namespace env
 
-def mk : env := dmap.mk
-def get (ref : reference) (m : env) : T ref.2 := @dmap.get reference (λ ref, T ref.2) _ _ ref m
-def insert (ref : reference) (x : T ref.2) (m : env) : env := @dmap.insert reference (λ ref, T ref.2) _ ref x m
-def has_key (ref : reference) (m : env) : Prop := dmap.has_key ref m
+def mk : env := quotient.mk (mk_hash_map reference.hash)
 
-instance decidable_has_key (ref : reference) (m : env) : decidable (has_key ref m) :=
-show decidable (dmap.has_key ref m), by tactic.apply_instance
+def get (ref : reference) (q : env) : T ref.2 := quotient.lift_on q
+(λ (m : pre_env),
+  match m^.find ref with
+  | none := default _
+  | some x := x
+  end)
+begin intros m₁ m₂ H_eqv, simp [H_eqv ref] end
+
+def insert (ref : reference) (x : T ref.2) (q : env) : env := quotient.lift_on q
+(λ (m : pre_env), quotient.mk $ m^.insert ref x)
+begin
+intros m₁ m₂ H_eqv, dsimp, apply quotient.sound,
+intros ref',
+cases (decidable.em (ref = ref')) with H_eq H_neq,
+simp [hash_map.find_insert, dif_ctx_simp_congr, H_eq, dif_pos],
+simp [hash_map.find_insert, dif_ctx_simp_congr, H_neq, dif_neg, H_eqv ref'],
+end
+
+def has_key (ref : reference) (q : env) : Prop := quotient.lift_on q
+(λ (m : pre_env), m^.contains ref)
+begin intros m₁ m₂ H_eqv, simp [hash_map.contains, H_eqv ref] end
 
 def get_ks : Π (refs : list reference) (m : env), dvec T refs^.p2
 | []          m := ⟦⟧
 | (ref::refs) m := dvec.cons (get ref m) (get_ks refs m)
 
 def insert_all : Π (refs : list reference) (vs : dvec T refs^.p2), env
-| []      ⟦⟧       := env.mk
+| []      ⟦⟧        := env.mk
 | (k::ks) (v:::vs) := env.insert k v (insert_all ks vs)
 
+-- Facts
 lemma has_key_insert {ref₁ ref₂ : reference} {x₂ : T ref₂.2} {m : env} :
-  has_key ref₁ m → has_key ref₁ (insert ref₂ x₂ m) := dmap.has_key_insert
+  has_key ref₁ m → has_key ref₁ (insert ref₂ x₂ m) :=
+assume H_contains_ref₁,
+begin
+induction m,
+dunfold has_key insert,
 
-lemma has_key_insert_diff {ref₁ ref₂ : reference} {x : T ref₂.2} {m : env} :
-  ref₁ ≠ ref₂ → has_key ref₁ (insert ref₂ x m) → has_key ref₁ m := sorry
+end
+
+
+
+
+end env
+end certigrad
+
+#exit
+
+
+
+
+-- We wrap `dmap` as `env` to avoid the need for higher-order unification.
+@[reducible] def env : Type := dmap reference (λ (ref : reference), T ref.2)
+
+namespace env
+
+instance decidable_has_key (ref : reference) (m : env) : decidable (has_key ref m) :=
+show decidable (dmap.has_key ref m), by tactic.apply_instance
+
+
 
 lemma has_key_insert_same (ref : reference) {x : T ref.2} (m : env) :
   has_key ref (insert ref x m) := dmap.has_key_insert_same ref m
@@ -54,16 +117,9 @@ lemma insert_insert_flip {ref₁ ref₂ : reference} (x₁ : T ref₁.2) (x₂ :
 lemma insert_insert_same (ref : reference) (x₁ x₂ : T ref.2) (m : env) :
   insert ref x₁ (insert ref x₂ m) = insert ref x₁ m := dmap.insert_insert_same ref x₁ x₂ m
 
-/-
-lemma nodup_insert {ref : reference} {x : T ref.2} {refs : list reference} {m : env} :
-  list.nodup (keys m ++ (ref :: refs)) → list.nodup (keys (insert ref x m) ++ refs) := dmap.nodup_insert
 
-lemma not_mem_of_insert {ref₀ ref : reference} {x : T ref.2} {refs : list reference} {m : env} :
-  ref₀ ∉ (keys m ++ (ref :: refs)) → ref₀ ∉ (dmap.keys (dmap.insert ref x m) ++ refs) := dmap.not_mem_of_insert
 
-lemma not_mem_of_insert_symm {ref₀ ref : reference} {x : T ref.2} {refs : list reference} {m : env} :
-  ref₀ ∉ (dmap.keys (dmap.insert ref x m) ++ refs) → ref₀ ∉ (keys m ++ (ref :: refs)) := dmap.not_mem_of_insert_symm
--/
+
 section proofs
 open list
 
@@ -123,11 +179,6 @@ lemma simp_has_key_insert_diff (ref₁ ref₂ : reference) {x : T ref₂.2} (m :
 
 lemma simp_has_key_empty (ref : reference) : has_key ref env.mk = false := sorry
 
---lemma simp_keys_nil : env.keys env.mk = [] := rfl
-
--- TODO(dhs): when I switch to hash-maps, this will be a little different
---lemma simp_keys_cons (ref : reference) (x : T ref.2) (m : env) : env.keys (env.insert ref x m) =
---list.insertion_sort has_lt.lt (ref :: env.keys m) := sorry
 
 
 
