src/certigrad/prove_model_ok.lean
@@ -186,7 +186,7 @@ attribute [cgsimp] dvec.head dvec.head2 dvec.head3
 attribute [cgsimp] integrate_kl integrate_mvn_iso_kl integrate_kl_pre integrate_mvn_iso_kl_pre reparameterize
 attribute [cgsimp] reparam reparameterize reparameterize_pre
 
-attribute [cgsimp] all_parents_in_env all_costs_scalars grads_exist_at pdfs_exist_at all_pre_satisfied
+attribute [cgsimp] all_parents_in_env all_costs_scalars grads_exist_at pdfs_exist_at all_pre_satisfied uniq_ids
                    is_gintegrable is_nabla_gintegrable is_gdifferentiable can_differentiate_under_integrals
 
 attribute [cgsimp] graph.to_dist operator.to_dist sum_costs compute_grad_slow
